## Swap Kth nodes from ends

Given a singly linked list of size N, and an integer K. You need to swap the Kth node from beginning and Kth node from the end in the linked list.  
Note: You need to swap the nodes through the links and not changing the content of the nodes.

#### Example 1:

```
Input:
N = 4,  K = 1
value[] = {1,2,3,4}
Output: 1
Explanation: Here K = 1, hence after
swapping the 1st node from the beginning
and end thenew list will be 4 2 3 1.
```

#### Example 2:

```
Input:
N = 5,  K = 3
value[] = {1,2,3,4,5}
Output: 1
Explanation: Here k = 3, hence after
swapping the 3rd node from the beginning
and end the new list will be 1 2 3 4 5.
```

#### Your Task:

The task is to complete the function `swapkthnode()`, which has arguments head, num(no of nodes), and K, and it should return a new head. The validation is done internally by the driver code to ensure that the swapping is done by changing references/pointers only. A correct code would always cause output as 1.

Expected Time Complexity: `O(n)`  
Expected Auxillary space Complexity: `O(1)`

```
Constraints:
1 <= N <= 10^3
1 <= K <= 10^3
```

```c++
/* Linked List Node structure
   struct Node  {
     int data;
     Node *next;
     Node(int x) {
        data = x;
        next = NULL;
  }
  }
*/
void print(Node* curr) {
    while(curr != NULL) {
        cout<<curr->data<<" ";
        curr = curr->next;
    }
    cout<<endl;
}

// Should swap Kth node from beginning and Kth
// node from end in list and return new head.
Node *swapkthnode(Node* head, int num, int K) {
    if(num == 1 || K > num)
        return head;
    if(K > num/2) {
        K = num - K +1;
    }
    if((num - K + 1) ==  K)
        return head;

    if(K == 1) {
        if(num == 2) {
            Node* next = head->next;
            head->next = NULL;
            next->next = head;
            return next;
        } else {
            Node* curr = head;
            while(curr->next->next != NULL) {
                curr = curr->next;
            }
            Node* tail = curr->next;
            curr->next = head;
            tail->next = head->next;
            head->next = NULL;
            return tail;
        }
    } else {
        if(K + 1 == num - K +1) {
            //The nodes are adjacent to each other
            Node* curr = head;
            int count = K-2;
            while(count--) {
                curr = curr->next;
            }
            Node* next = curr->next;
            curr->next = curr->next->next;
            next->next = curr->next->next;
            curr->next->next = next;
        } else {
            Node* curr1 = head;
            Node* curr2 = head;
            int count1 = K-2, count2 = num-K-1;
            while(count1--)
                curr1 = curr1->next;
            while(count2--)
                curr2 = curr2->next;

            Node* next = curr1->next;
            Node* nextTonext = curr1->next->next;
            curr1->next = curr2->next;
            next->next = curr1->next->next;
            curr2->next = next;
            curr1->next->next = nextTonext;
        }
        return head;
    }
}
```
